CollapsingTowers/TwoLevelMut/SyntacticTyping/Defs.lean
@@ -1,3 +1,4 @@
+import CollapsingTowers.TwoLevelMut.SyntacticTyping.Meta
 import CollapsingTowers.TwoLevelMut.SyntacticTyping.Effect
 import CollapsingTowers.TwoLevelMut.SyntacticTyping.Ty
 import CollapsingTowers.TwoLevelMut.SyntacticTyping.Env
