CollapsingTowers/TwoLevelMut/SyntacticTyping/Meta.lean
@@ -1,0 +1,58 @@
+import Mathlib.Order.Basic
+
+inductive Meta : Type where
+  | pure
+  | reify
+
+notation:max "⊥" => Meta.pure
+
+notation:max "⊤" => Meta.reify
+
+@[simp]
+def Meta.union : Meta → Meta → Meta
+  | ⊥, ⊥ => ⊥
+  | ⊤, _ => ⊤
+  | _, ⊤ => ⊤
+
+@[simp]
+instance : Union Meta where union := Meta.union
+
+@[simp]
+lemma Meta.union_pure : forall φ : Meta, φ ∪ ⊥ = φ := by
+  intro φ
+  cases φ <;> rfl
+
+@[simp]
+lemma Meta.pure_union : forall φ : Meta, ⊥ ∪ φ = φ := by
+  intro φ
+  cases φ <;> rfl
+
+@[simp]
+lemma Meta.union_reify : forall φ : Meta, φ ∪ ⊤ = ⊤ := by
+  intro φ
+  cases φ <;> rfl
+
+@[simp]
+lemma Meta.reify_union : forall φ : Meta, ⊤ ∪ φ = ⊤ := by
+  intro φ
+  cases φ <;> rfl
+
+@[simp]
+def Meta.le : Meta → Meta → Prop
+  | ⊥, _ => true
+  | ⊤, ⊤ => true
+  | _, _ => false
+
+@[simp]
+instance : LE Meta where le := Meta.le
+
+instance : Preorder Meta where
+  le_refl := by intro x; cases x <;> simp
+  le_trans := by intros x y z; cases x <;> cases y <;> cases z <;> simp
+  lt_iff_le_not_ge := by intros x y; cases x <;> cases y <;> simp
+
+instance : PartialOrder Meta where
+  le_antisymm := by
+    intros x y
+    cases x <;> cases y <;> simp
+    all_goals intro _ _; contradiction
